Challenge/Ripemd160/Submission/Proofs/Bytecode/StackRoundData.lean
@@ -60,19 +60,19 @@ def rightConstant (i : Nat) : UInt256 :=
 
 def leftHelperPCOfGroup (group : Nat) : UInt256 :=
   match group with
-  | 0 => UInt256.ofNat 0xfb3
-  | 1 => UInt256.ofNat 0xfe7
-  | 2 => UInt256.ofNat 0xe4b
-  | 3 => UInt256.ofNat 0x107e
-  | _ => UInt256.ofNat 0x10ce
+  | 0 => UInt256.ofNat 0xfb9
+  | 1 => UInt256.ofNat 0xfed
+  | 2 => UInt256.ofNat 0xe51
+  | 3 => UInt256.ofNat 0x1084
+  | _ => UInt256.ofNat 0x10d4
 
 def rightHelperPCOfGroup (group : Nat) : UInt256 :=
   match group with
-  | 0 => UInt256.ofNat 0xeed
-  | 1 => UInt256.ofNat 0x1135
-  | 2 => UInt256.ofNat 0xf5f
-  | 3 => UInt256.ofNat 0xf9f
-  | _ => UInt256.ofNat 0xfb6
+  | 0 => UInt256.ofNat 0xef3
+  | 1 => UInt256.ofNat 0x113b
+  | 2 => UInt256.ofNat 0xf65
+  | 3 => UInt256.ofNat 0xfa5
+  | _ => UInt256.ofNat 0xfbc
 
 def leftHelperPC (i : Nat) : UInt256 :=
   leftHelperPCOfGroup (i / 16)
